Obten el resultado de las siguientes operaciones tomando en cuenta la \textbf{jerarquía de operaciones}.

\begin{multicols}{2}
    \begin{parts}
        \part $9\times10+3=$\fillin[93][1.5cm]

        \begin{solutionbox}{2.2cm}

        \end{solutionbox}

        \part $6-2\left(5-3+1\right)=$\fillin[0][1.5cm]

        \begin{solutionbox}{2.2cm}
            \[
                \begin{array}{rlr}
                     & =6-2\left(5-3+1\right) & \text{\scriptsize Suma dentro del paréntesis} \\
                     & =6-2\times 3           & \text{\scriptsize Multiplica 2 y 3}           \\
                     & =6-6                   & \text{\scriptsize Resta 6 y 6}                \\
                     & =0                     &
                \end{array}
            \]
        \end{solutionbox}

        \part $4-1\times2=$\fillin[2][1.5cm]

        \begin{solutionbox}{2.2cm}

        \end{solutionbox}

        \part $2+12 \div 2\times3=$\fillin[2][1.5cm]

        \begin{solutionbox}{2.2cm}

        \end{solutionbox}

        \part $3\times9+10\times\dfrac{36}{6}=$\fillin[87][1.5cm]

        \begin{solutionbox}{2.2cm}

        \end{solutionbox}

        \part $9-3\times2=$\fillin[3][1.5cm]

        \begin{solutionbox}{2.2cm}

        \end{solutionbox}

        \part $6\times4+2\times3=$\fillin[30][1.5cm]

        \begin{solutionbox}{2.2cm}
            \[
                \begin{array}{rlr}
                     & =6\times 4+2\times 3 & \text{\scriptsize Multiplica 6 y 4} \\
                     & =24+2\times 3        & \text{\scriptsize Multiplica 2 y 3} \\
                     & =24+6                & \text{\scriptsize Suma 24 y 6}      \\
                     & =30                  &
                \end{array}
            \]
        \end{solutionbox}


        \part $8 \div 4-\left(-10+8\right)=$\fillin[2][1.5cm]

        \begin{solutionbox}{2.2cm}

        \end{solutionbox}
    \end{parts}
\end{multicols}