\part[10] $y=-6x^2 +384$
\fullwidth{
    \begin{solutionbox}{11cm}
        \begin{multicols}{2}
            Por factorización:
            \[
                \begin{array}{rl}
                    y          & =	      -6x^2 +384              \\
                               & \text{Ya que $y=0$, entonces } \\
                    0          & =	      -6x^2 +384              \\
                    0          & =		 -6(x^2 -64)                  \\
                    0          & =		 -6(x - 8)(x + 8)             \\
                    0          & =	       -6(x - 8)(x + 8)       \\
                    \therefore & x_1 =-8 \text{ y } x_2 =8
                \end{array}
            \]
            \\
            Por despeje:
            \[
                \begin{array}{rl}
                    y             & =	 -6x^2 +384                   \\
                                  & \text{Ya que $y=0$, entonces } \\
                    0             & =	  -6x^2 +384                  \\
                    -384          & =	  -6x^2                       \\
                    384           & =	  6x^2                        \\
                    64            & =	  x^2                         \\
                    \pm \sqrt{64} & =	  x                           \\
                    \pm 8         & =	  x                           \\
                    \therefore    & x_1 =-8 \text{ y } x_2 =8
                \end{array}
            \]
            \\
            Por fórmula general:
            \[
                \begin{array}{rl}
                    y          & =	      -6x^2 +384
                    \\
                    a          & =-6
                    \\
                    b          & =0
                    \\
                    c          & =384
                    \\
                    x_{1,2}    & = \dfrac{-b\pm\sqrt{b^2-4ac}}{2a}
                    \\[2em]
                    x_{1,2}    & = \dfrac{0\pm\sqrt{0^2-4(-6)(384)}}{2(-6)}
                    \\[2em]
                    x_{1,2}    & = \dfrac{\pm\sqrt{9216}}{-12}
                    \\[2em]
                    x_{1,2}    & = \dfrac{\pm96}{-12}
                    \\[2em]
                    \therefore & x_1 =\dfrac{96}{-12}=-8 \text{ y }  x_2
                    =\dfrac{-96}{-12}=8                                     \\[2em]
                \end{array}
            \]
        \end{multicols}
    \end{solutionbox}
}