\part $x^2+12x+36=0$

\begin{solutionbox}{10cm}
    \begin{multicols}{2}
        Por factorización:
        \[
            \begin{array}{rl}
                x^2+12x+36 & = 0          \\
                (x+6)(x+6) & = 0          \\
                \therefore & x_1 =x_2 =-6
            \end{array}
        \]
        \\
        Por fórmula general:
        \[
            \begin{array}{rl}
                y          & =	      x^2+12x+36
                \\
                a          & =1
                \\
                b          & =12
                \\
                c          & =36
                \\
                x_{1,2}    & = \dfrac{-b\pm\sqrt{b^2-4ac}}{2a}
                \\[2em]
                x_{1,2}    & = \dfrac{-(12)\pm\sqrt{(12)^2-4(1)(36)}}{2(1)}
                \\[2em]
                x_{1,2}    & = \dfrac{-12\pm\sqrt{0}}{2}
                \\[2em]
                x_{1,2}    & = \dfrac{-12\pm 0}{2}
                \\[2em]
                \therefore & x_1 =x_2=\dfrac{-12}{2}=-6
            \end{array}
        \]
    \end{multicols}
\end{solutionbox}
